

Q1)
\uline{Système} : \{ S(\textit{m}) \}
\hskip 5em
\uline{Référentiel} : Géocentrique

\vspace{2em}

\uline{RFD} \hskip 1em $\sum \mathbf{F} = m\mathbf{a}$
$\quad \Rightarrow \quad$
$\displaystyle
\frac {dv} {dt} \mathbf{T} + \frac {v^2} {r} \mathbf{N} = \frac {GM} {r^2} \mathbf {N}$

\vspace{1em}
D'où $\displaystyle v^2 = \frac {GM} {r}$,
et donc $\displaystyle \mathcal{E}_c = \frac {1} {2} \frac {GMm} {r}$

\vspace{1em}
Or, $\displaystyle \mathcal{E}_p = -\frac {GMm} {r}$,
d'où $\boxed {2\mathcal{E}_c + \mathcal{E}_p = 0}$

\vspace{1em}
Q2) a) Sur un tour complet :
\begin{align*}
\Delta\mathcal{E}_m &= \Delta\mathcal{E}_c + \Delta\mathcal{E}_p \\
 &= \frac {1} {2} m\left( v_f^2-v_i^2\right) - GMm\left(\frac {1} {R-\varepsilon} - \frac {1} {\varepsilon}\right) \\
 &= \frac {1} {2} GMm\left(\frac {1} {R-\varepsilon} - \frac {1} {\varepsilon}\right) - GMm\left(\frac {1} {R-\varepsilon} - \frac {1} {\varepsilon}\right) \\
 &= -\frac {1} {2} \frac {GMm} {R} \left(\frac {1} {1- \frac{\varepsilon} {R}} - 1\right) \\
 &\approx -\frac {1} {2} \frac {GMm\varepsilon} {R^2}
\end{align*}

Or,
$\displaystyle \mathcal{W}(\mathbf{F_f}) = \int \mathbf{F}\cdot \mathbf{dl}
=\int -\alpha mv\mathbf{v}\cdot\mathbf{dl}
\approx-2\pi R\alpha mv^2$

\vspace{1em}
D'où \uline{TEM} : $\displaystyle \Delta \mathcal{E}_m = \mathcal{W(\mathbf{F_f})}
\Leftrightarrow \boxed {\alpha = \frac {\varepsilon} {4\pi R^2}}$

\vspace{1em}
b) $\displaystyle T= \frac {v} {d} = \sqrt {\frac {GM} {R}} \frac {1} {2\pi R}
= \sqrt {\frac {GM} {4\pi^2}} \frac {1} {R^{-3/2}}$

\vspace{1em}
Donc plus généralement, $\displaystyle T_n = K(R-\varepsilon n)^{-3/2}$, où $\displaystyle K = \sqrt {\frac {GM} {4\pi^2}}$

\vspace{1em}
\uline{DL} : $\displaystyle T_n = KR^{-3/2}\left(1-\frac {\varepsilon n} {R}\right)^{-3/2}
\approx KR^{-3/2}\left(1+ \frac {3} {2} \frac {\varepsilon n} {R}\right)$

\vspace{1em}
Donc :
\begin{align*}
\sum_{k=0}^{n} T_k = T_{p} \quad &\Leftrightarrow \quad KR^{-3/2} \sum_{k=0}^{n}\left(1 +\frac {3} {2} \frac {\varepsilon n} {R}\right) = T_p \\
&\Leftrightarrow \quad U\left(n + 1 + \frac {3} {2} \frac {\varepsilon} {R} \frac {n(n+1)} {2} \right) = 1 \quad \left(U = \frac {KR^{-3/2}} {T_p}\right) \\
&\Leftrightarrow \quad n^2 + n\left(\frac {4} {3} \frac {R} {\varepsilon} + 1\right) + \frac {4} {3} \frac {R} {\varepsilon} - \frac {1} {U} = 0 \\
&\Leftrightarrow \quad n^2 + \frac {4} {3} \frac {R} {\varepsilon}n - \frac {1} {U} = 0 \\
\end{align*}
\uline{AN} : $n \approx 2\cdot 10^5$, donc $\displaystyle \boxed {h \approx 200 \; km}$
